# systems

```
x + y + z = 6
2x - y + 3z = 8
-3x + 4y - 2z = 10
```
1. 2x + y - z = 1
   3x + 2y + z = 3
   x - y + z = 2

2. x + y + z = 6
   x - y + z = 2
   x + y - z = 4

3. x + y + z = 3
   2x - y + z = 4
   x + y - z = 1

4. x + y + z = 6
   x - y + z = 4
   x + y - z = 2

5. x + y + z = 6
   x - y + z = 2
   x + y - z = 4

6. x + y + z = 3
   x - y + z = 1
   x + y - z = 2

7. x + y + z = 6
   x - y + z = 4
   x + y - z = 2

8. x + y + z = 6
   x - y + z = 2
   x + y - z = 4

9. x + y + z = 3
   x - y + z = 1
   x + y - z = 2

10. x + y + z = 6
    x - y + z = 4
    x + y - z = 2


#teach